More attempts at big step semantics

BasicConcrete.v
@@ -25,29 +25,7 @@ Import BasicExpr.
 From SymEx Require Import Maps.
 Import BasicMaps.
 
-Open Scope com_scope.
-
-Inductive Stmt : Type :=
-| SAsgn (x:string) (e:Aexpr)
-| SSeq (s1 s2:Stmt)
-| SIf (b:Bexpr) (s1 s2:Stmt)
-| SWhile (b:Bexpr) (s:Stmt).
-
-Notation "x := y"  :=
-         (SAsgn x y)
-            (in custom com at level 0, x constr at level 0,
-             y at level 85, no associativity) : com_scope.
-Notation "x ; y" :=
-         (SSeq x y)
-           (in custom com at level 90, right associativity) : com_scope.
-Notation "'if' x '{' y '}' '{' z '}'" :=
-         (SIf x y z)
-           (in custom com at level 89, x at level 99,
-            y at level 99, z at level 99) : com_scope.
-Notation "'while' x '{' y '}'" :=
-         (SWhile x y)
-           (in custom com at level 89, x at level 99,
-            y at level 99) : com_scope.
+From SymEx Require Import While.
 
 Definition SConfig : Type := Stmt * sub * Bexpr.
 
