BigStep.v
@@ -1,0 +1,411 @@
+From Coq Require Import
+                 Strings.String
+                 Bool.Bool
+                 Init.Datatypes
+                 Lists.List
+                 Psatz
+                 ZArith
+                 Ensembles
+                 Classes.RelationClasses.
+
+From SymEx Require Import Expr.
+Import BasicExpr.
+
+From SymEx Require Import Maps.
+Import BasicMaps.
+
+From SymEx Require Import While.
+Open Scope com_scope.
+
+(** Trying the Nakata & Uustalu approach (functional big-step concrete/symbolic semantics)*)
+
+CoInductive trace {X:Type}: Type :=
+| TNil: X -> @trace X
+| TCons: X -> @trace X -> @trace X.
+
+CoInductive infinite {X:Type}: @trace X -> Prop :=
+  | inf_intro: forall t x, infinite t -> infinite (TCons x t).
+
+CoInductive trace_bisim {X: Type}: @trace X -> @trace X -> Prop :=
+| bisim_singl: forall x x': X, trace_bisim (TNil x) (TNil x)
+| bisim_step: forall t t' x, trace_bisim t t' -> trace_bisim (TCons x t) (TCons x t').
+
+Global Instance trace_bisim_refl {X: Type}: Reflexive (@trace_bisim X).
+Proof. cofix CH; intros x; destruct x.
+       - constructor. exact x.
+       - constructor. apply CH.
+Qed.
+
+Global Instance trace_eq_sym {X: Type}: Symmetric (@trace_bisim X).
+Proof.
+  cofix CH; intros x y H. destruct x, y;
+    try (inversion H; subst; assumption).
+  inversion H; subst. constructor. apply (CH _ _ H1).
+Qed.
+
+Global Instance trace_eq_trans {X: Type}: Transitive (@trace_bisim X).
+Proof.
+  cofix CH; intros x y z H0 H1. destruct x, y, z;
+    try (inversion H0; inversion H1; subst; assumption).
+  inversion H1; subst; inversion H0; subst. constructor.
+  apply (CH x0 y z H3 H2).
+Qed.
+
+Notation " t '~' t'" := (trace_bisim t t')
+                        (at level 40).
+
+Definition unfold_trace {X} (t: @trace X): @trace X :=
+         match t with
+        | TNil x => TNil x
+        | TCons x t => TCons x t
+         end.
+
+Lemma unfold_id {X}: forall (t: @trace X), t = unfold_trace t.
+Proof. destruct t; reflexivity. Qed.
+
+Inductive last_state {X:Type}: @trace X -> X -> Prop :=
+| Last: forall x, last_state (TNil x) x
+| Not_last:  forall t x x', last_state t x -> last_state (TCons x' t) x.
+
+Lemma last_state_inf {X: Type}: forall t, (~ exists (x: X), last_state t x) -> infinite t.
+Proof.
+    cofix CH. intros.
+    destruct t.
+    + exfalso.
+      apply H.
+      exists x. constructor.
+    + constructor.
+      apply CH. intro contra.
+      apply H. destruct contra as [x0 Hlast].
+      exists x0. constructor. apply Hlast.
+Qed.
+
+CoFixpoint append {X: Type} (t1 t2: @trace X): @trace X :=
+         match t1 with
+        | TNil x => TCons x t2
+        | TCons x t => TCons x (append t t2)
+         end.
+Notation " t '+++' t'" := (append t t')
+                        (at level 40).
+
+Lemma append_nil {X: Type}: forall (x: X) t, TNil x +++ t = TCons x t.
+Proof. intros. rewrite (unfold_id (TNil x +++ t)). reflexivity. Qed.
+
+Lemma append_cons {X: Type}: forall (x: X) t t', TCons x t +++ t' = TCons x (t +++ t').
+Proof. intros. rewrite (unfold_id (TCons x t +++ t')). reflexivity. Qed.
+
+CoFixpoint repeat_trace {X:Type} (x: X): @trace X := TCons x (repeat_trace x).
+
+(* Concrete Big-Step Functional Semantics *)
+Definition trace__C := @trace Valuation.
+
+CoFixpoint sequence (k: Valuation -> trace__C) (t: trace__C): trace__C :=
+  match t with
+  (* This makes it so eval <{p ; q}> ~ eval p +++ eval q*)
+  | TNil V => TCons V (k V)
+  | TCons V t' => TCons V (sequence k t')
+  end.
+
+Lemma eval_seq_nil: forall k V, sequence k (TNil V) = TCons V (k V).
+Proof. intros. rewrite (unfold_id (sequence k (TNil V))), (unfold_id (TCons V (k V))). reflexivity. Qed.
+
+Lemma eval_seq_cons: forall k V t, sequence k (TCons V t) = TCons V (sequence k t).
+Proof. intros. rewrite unfold_id with (t := sequence k (TCons V t)). reflexivity. Qed.
+
+CoFixpoint loop (k: Valuation -> trace__C) (p: Valuation -> bool) (V: Valuation): trace__C :=
+  if p V then
+    match k V with
+    | TNil V' => TCons V' (loop k p V')
+    | TCons V' t => TCons V' (loopseq k p t)
+    end
+  else TNil V
+with loopseq (k: Valuation -> trace__C) (p: Valuation -> bool) (t: trace__C): trace__C :=
+       match t with
+       | TNil V => TCons V (loop k p V)
+       | TCons V t' => TCons V (loopseq k p t')
+       end.
+
+Lemma loopseq_nil: forall k p V, loopseq k p (TNil V) = TCons V (loop k p V).
+Proof. intros. rewrite unfold_id with (t := loopseq k p (TNil V)). reflexivity. Qed.
+
+Lemma loopseq_cons: forall k p V t, loopseq k p (TCons V t) = TCons V (loopseq k p t).
+Proof. intros. rewrite unfold_id with (t := loopseq k p (TCons V t)). reflexivity. Qed.
+
+Lemma loopseq_append: forall k p t V, last_state t V -> (loopseq k p t) ~ (t +++ loop k p V).
+Proof.
+    cofix CH. intros.
+    rewrite unfold_id with (t := loopseq k p t).
+    rewrite unfold_id with (t := t +++ loop k p V).
+    destruct t.
+    - inversion H; subst. reflexivity.
+    - simpl. constructor.
+      apply CH. inversion H; assumption.
+Qed.
+
+Fixpoint eval (p:Stmt) (V:Valuation): trace__C :=
+  match p with
+  | <{skip}> => TNil V
+  | <{x := e}> => TNil (x !-> Aeval V e ; V)
+  | <{p ; q}> => sequence (eval q) (eval p V)
+  | <{if e {p} {q}}> => if Beval V e then eval p V else eval q V
+  | <{while e {p}}> => (loop (eval p) (fun V => Beval V e) V)
+  end.
+
+(* Ideally I'd have
+eval__C (p: Stmt): Valuation -> Valuation := fun V => last_state (eval p V)
+but that assumes decidability
+ *)
+
+Example ex1: eval <{X := 4}> (_ !-> 0) = TNil (X !-> 4 ; _ !-> 0) := eq_refl.
+Example ex2: eval <{X := 4 ; Y := 2}> (_ !-> 0) = TCons (X !-> 4 ; _ !-> 0) (TNil (Y !-> 2 ; X !-> 4 ; _ !-> 0)).
+Proof.
+    simpl.
+    rewrite unfold_id with (t := sequence (fun V : Valuation => TNil (Y !-> 2; V)) (TNil (X !-> 4; _ !-> 0))).
+    rewrite unfold_id with (t := (TNil (Y !-> 2; X !-> 4; _ !-> 0))).
+    reflexivity.
+Qed.
+Example ex3: eval <{if X <= 1 {Y := 4} {Y := 2}}> (_ !-> 0) = (TNil (Y !-> 4 ; _ !-> 0)) :=
+         eq_refl.
+Example ex4: eval <{if X <= 1 {Y := 4} {Y := 2}}> (_ !-> 2) = (TNil (Y !-> 2 ; _ !-> 2)) :=
+         eq_refl.
+Example ex5: eval <{while X <= 1 {X := X + 1}}> (_ !-> 0)
+             = (TCons (X !-> 1 ; _ !-> 0) (TCons (X !-> 2 ; X !-> 1 ; _ !-> 0) (TNil (X !-> 2 ; X !-> 1 ; _ !-> 0)))).
+Proof.
+    simpl.
+    rewrite unfold_id with (t := (loop (fun V => TNil (X !-> V X + 1; V)) (fun V => V X <=? 1) (_ !-> 0))).
+    simpl.
+    rewrite unfold_id with (t := (loop (fun V => TNil (X !-> V X + 1; V)) (fun V => V X <=? 1) (X !-> 1; _ !-> 0))).
+    simpl.
+    rewrite unfold_id with (t := (loop (fun V => TNil (X !-> V X + 1; V)) (fun V => V X <=? 1) (X !-> 2; X !-> 1; _ !-> 0))).
+    reflexivity.
+Qed.
+
+(* note that this is not an equality *)
+Example ex6: eval <{while X <= 1 { skip }}> (_ !-> 0) ~ repeat_trace (_ !-> 0).
+Proof.
+    cofix CH.
+    simpl in *.
+    rewrite unfold_id with (t := repeat_trace (_ !-> 0)).
+    rewrite unfold_id with (t := (loop (fun V => TNil V) (fun V => V X <=? 1) (_ !-> 0))).
+    simpl. constructor.
+    apply CH.
+Qed.
+
+Lemma seq_append': forall t k V,
+    last_state t V ->
+    sequence k t ~ (t +++ k V).
+Proof.
+    cofix CH. intros.
+    rewrite unfold_id with (t := sequence k t).
+    rewrite unfold_id with (t := t +++ k V).
+    destruct t.
+    - simpl. inversion H; subst.
+      reflexivity.
+    - simpl. constructor. apply CH.
+      inversion H; subst. apply H3.
+Qed.
+
+Lemma seq_append: forall p1 p2 V V',
+    last_state (eval p1 V) V' ->
+    (sequence (eval p2) (eval p1 V)) ~ ((eval p1 V) +++ (eval p2 V')).
+Proof. intros.
+       apply seq_append'.
+       apply H.
+Qed.
+
+Lemma seq_append_eval: forall p1 p2 V V',
+    last_state (eval p1 V) V' ->
+    (eval <{p1 ; p2}> V) ~ ((eval p1 V) +++ (eval p2 V')).
+Proof. intros. simpl. apply seq_append. assumption. Qed.
+
+Example loop_sanity_ex: eval <{while X <= 1 {X := X + 1}}> (_ !-> 0)
+                     = eval <{if X <= 1 {X := X + 1} {skip} ; while X <= 1 {X := X + 1}}> (_ !-> 0).
+Proof.
+    simpl.
+    rewrite unfold_id with (t := loop (fun V : Valuation => TNil (X !-> V X + 1; V)) (fun V : Valuation => V X <=? 1) (_ !-> 0)).
+    rewrite unfold_id with (t := sequence (fun V : Valuation => loop (fun V0 : Valuation => TNil (X !-> V0 X + 1; V0)) (fun V0 : Valuation => V0 X <=? 1) V) (TNil (X !-> 1; _ !-> 0))).
+    simpl.
+    reflexivity.
+Qed.
+
+(* this is not actually true since sequencing adds a stutter step when case is false *)
+(* Lemma loop_sanity: forall p e V, *)
+(*     eval <{while e {p}}> V ~ eval <{if e {p} {skip} ; while e {p}}> V. *)
+
+(*The same approach will not work for symbolic execution because non-determinism
+  in "Coinductive Big-Step Semantics for Concurrency" they handle non-determinism with resumptions,
+  let's do something similar?
+ *)
+(* this is very C-trees, actually*)
+CoInductive tree__S: Type :=
+  | ret (_:sub): tree__S
+  | delay (_:sub) (_:tree__S): tree__S
+  | choice (_: Bexpr) (_ _: tree__S): tree__S.
+
+Lemma unfold_tree: forall t,
+    t = match t with
+       | ret s => ret s
+       | delay s t' => delay s t'
+       | choice b t1 t2 => choice b t1 t2
+        end.
+Proof. intros. destruct t; reflexivity. Qed.
+
+CoInductive tree_bisim: tree__S -> tree__S -> Prop :=
+  | ret_bisim: forall s, tree_bisim (ret s) (ret s)
+  | delay_bisim: forall s t t', tree_bisim t t' -> tree_bisim (delay s t) (delay s t')
+  | choice_bisim: forall b t1 t1' t2 t2',
+      tree_bisim t1 t1' ->
+      tree_bisim t2 t2' ->
+      tree_bisim (choice b t1 t2) (choice b t1' t2')
+.
+
+Notation " t '~~' t'" := (tree_bisim t t')
+                        (at level 40).
+
+CoInductive in_tree__S: tree__S -> sub -> Bexpr -> Prop :=
+  | In_leaf: forall s,
+      in_tree__S (ret s) s BTrue
+  | In_delay: forall s s' b t,
+      in_tree__S t s b -> in_tree__S (delay s' t) s b
+  | In_left: forall s b b' t1 t2,
+      in_tree__S t1 s b -> in_tree__S (choice b' t1 t2) s <{b' && b}>
+  | In_right: forall s b b' t1 t2,
+      in_tree__S t2 s b -> in_tree__S (choice b' t1 t2) s <{~ b' && b}>
+.
+
+CoFixpoint sequence__S (k: sub -> tree__S) (t: tree__S): tree__S :=
+         match t with
+        | ret s => k s
+        | delay s t' => delay s (sequence__S k t')
+        | choice b t1 t2 => choice b (sequence__S k t1) (sequence__S k t2)
+         end.
+
+CoFixpoint evalbranch__S (p: Stmt) (t: tree__S): tree__S :=
+         match t with
+        | ret s => ret s
+        | delay s t' => delay s (evalbranch__S p t')
+        | choice b t1 t2 => choice b (evalbranch__S p t1) (evalbranch__S p t2)
+         end.
+
+CoFixpoint loop__S (k: sub -> tree__S) (b: Bexpr) (s: sub): tree__S :=
+         choice b
+         (match k s with
+         | ret s' => delay s' (loop__S k b s')
+         | delay s t => delay s (loopseq__S k b t)
+         | choice b' t1 t2 => choice b' (loopseq__S k b t1) (loopseq__S k b t2)
+          end)
+         (ret s)
+with loopseq__S (k: sub -> tree__S) (b: Bexpr) (t: tree__S): tree__S :=
+       match t with
+      | ret s => delay s (loop__S k b s)
+      | delay s t' => delay s (loopseq__S k b t')
+      | choice b' t1 t2 => choice b' (loopseq__S k b t1) (loopseq__S k b t2)
+       end.
+
+Fixpoint eval__S (p:Stmt) (s: sub): tree__S :=
+  match p with
+  | <{skip}> => ret s
+  | <{x := e}> => ret (x !-> Aapply s e ; s)
+  | <{p ; q}> => sequence__S (eval__S q) (eval__S p s)
+  | <{if e {p} {q}}> => choice e (evalbranch__S q (eval__S p s)) (evalbranch__S p (eval__S q s))
+  | <{while e {p}}> => choice e (evalbranch__S SSkip (loop__S (eval__S p) e s)) (ret s)
+  end.
+
+Example ex1__S: eval__S <{X := 4}> id_sub = ret (X !-> 4 ; id_sub).
+Proof. reflexivity. Qed.
+
+Example ex2__S: eval__S <{X := 4 ; Y := 2}> id_sub = ret (Y !-> 2 ; X !-> 4 ; id_sub).
+Proof.
+    simpl.
+    rewrite unfold_tree with (t := sequence__S (fun s : sub => ret (Y !-> 2; s)) (ret (X !-> 4; id_sub))).
+    reflexivity.
+Qed.
+
+Example ex3__S: eval__S <{if X <= 1 {Y := 4} {Y := 2}}> id_sub = choice <{X <= 1}> (ret (Y !-> 4 ; id_sub)) (ret (Y !-> 2 ; id_sub)).
+Proof.
+    simpl.
+    rewrite unfold_tree with (t := (evalbranch__S <{ Y := 2 }> (ret (Y !-> 4; id_sub)))).
+    rewrite unfold_tree with (t := (evalbranch__S <{ Y := 4 }> (ret (Y !-> 2; id_sub)))).
+    reflexivity.
+Qed.
+
+Example ex4__S: eval__S <{if X <= 1 {Y := 4 ; Z := 4} {Y := 2} ; X := Y + 1}> id_sub
+              = choice <{X <= 1}> (ret (X !-> <{4 + 1}>; Z !-> 4; Y !-> 4 ; id_sub)) (ret (X !-> <{2 + 1}> ; Y !-> 2; id_sub)).
+Proof.
+    simpl.
+    rewrite unfold_tree with (t := sequence__S (fun s : sub => ret (X !-> APlus (s Y) 1; s))
+    (choice <{ X <= 1 }> (evalbranch__S <{ Y := 2 }> (sequence__S (fun s : sub => ret (Z !-> 4; s)) (ret (Y !-> 4; id_sub))))
+                        (evalbranch__S <{ Y := 4; Z := 4 }> (ret (Y !-> 2; id_sub))))).
+    simpl.
+    rewrite unfold_tree with (t := (sequence__S (fun s : sub => ret (X !-> APlus (s Y) 1; s))
+                                    (evalbranch__S <{ Y := 2 }> (sequence__S (fun s : sub => ret (Z !-> 4; s)) (ret (Y !-> 4; id_sub)))))).
+    simpl.
+    rewrite unfold_tree with (t := (sequence__S (fun s : sub => ret (X !-> APlus (s Y) 1; s))
+                                    (evalbranch__S <{ Y := 4; Z := 4 }> (ret (Y !-> 2; id_sub))))).
+    simpl.
+    replace ((Z !-> 4 ; Y !-> 4 ; id_sub) Y) with (AConst 4).
+    replace ((Y !-> 2; id_sub) Y) with (AConst 2).
+    all: reflexivity.
+Qed.
+
+(**
+CoFixpoint loop_tree (k: sub -> tree__S) (b: Bexpr) (s: sub): tree__S :=
+         choice b (loop_tree k b s) (ret s).
+(* should update s somehow *)
+
+Example ex5__S: eval__S <{while X <= 1 {X := X + 1}}> id_sub ~~ loop_tree (eval__S <{X := X + 1}>) <{X <= 1}> id_sub.
+Proof.
+    simpl.
+    cofix CH.
+    rewrite unfold_tree with (t := (evalbranch__S <{ skip }> (loop__S (fun s : sub => ret (X !-> APlus (s X) 1; s)) <{ X <= 1 }> id_sub))).
+    rewrite unfold_tree with (t := (loop__S (fun s : sub => ret (X !-> APlus (s X) 1; s)) <{ X <= 1 }> id_sub)) in *.
+    simpl in *.
+    rewrite unfold_tree with (t := (evalbranch__S <{ skip }> (ret id_sub))).
+    rewrite unfold_tree with (t := loop_tree (fun s => ret (X !-> APlus (s X) 1; s)) <{ X <= 1 }> id_sub).
+    simpl. constructor.
+    - inversion CH; subst.
+      constructor.
+    - constructor.
+Qed.
+*)
+
+Lemma correctness: forall p V F B,
+    in_tree__S (eval__S p id_sub) F B ->
+    Beval V B = true ->
+    last_state (eval p V) (Comp V F).
+Proof.
+    induction p; intros; simpl.
+    - inversion H; subst. rewrite comp_id. apply Last.
+    - inversion H; subst.
+      rewrite asgn_sound, comp_id. apply Last.
+    - admit.
+    - inversion H; subst;
+        simpl in H0; apply andb_true_iff in H0; destruct H0;
+        destruct (Beval V b);
+        try discriminate.
+      + eapply IHp1.
+        apply (IHp1 _ _ _ H6 H1).
+      + apply Not_last. apply (IHp2 _ _ _ H6 H1).
+    - inversion H; subst.
+      + admit. (* bad form of loop *)
+      + admit.
+      + admit.
+
+Lemma completeness: forall p V V',
+    last_state (eval p V) V' ->
+    exists F B, in_tree__S (eval__S p id_sub) F B
+           /\ V' = Comp V F
+           /\ Beval V B = true.
+Proof.
+    induction p; simpl; intros.
+    - exists id_sub. exists BTrue. repeat split.
+      + constructor.
+      + inversion H; subst. apply comp_id.
+    - exists (x !-> Aapply id_sub e; id_sub) . exists BTrue. repeat split.
+      + constructor.
+      + inversion H; subst.
+        rewrite asgn_sound. rewrite comp_id.
+        reflexivity.
+    - inversion H; subst.
+      + rewrite unfold_id with (t := sequence (eval p2) (eval p1 V)) in H1.
+        simpl in H1.
