BigStepClassical.v
@@ -1,0 +1,446 @@
+From Coq Require Import
+                 Strings.String
+                 Bool.Bool
+                 Init.Datatypes
+                 Lists.List
+                 Psatz
+                 ZArith
+                 Ensembles
+                 Classes.RelationClasses.
+
+From SymEx Require Import Expr.
+Import BasicExpr.
+
+From SymEx Require Import Maps.
+Import BasicMaps.
+
+From SymEx Require Import While.
+Open Scope com_scope.
+
+(* blæh *)
+From Coq Require Import Classical Description.
+
+(* Trick from Leroy *)
+Inductive lessdef {A: Type}: option A -> option A -> Prop :=
+  | lessdef_none: forall oa, lessdef None oa
+  | lessdef_some: forall a, lessdef (Some a) (Some a).
+
+Notation "x <<= y" := (lessdef x y) (at level 70, no associativity).
+
+Lemma lessdef_refl {X:Type}: forall (x:option X), x <<= x.
+Proof. destruct x; constructor. Qed.
+
+#[export]
+Hint Constructors lessdef : lessdef.
+
+Section LIMIT.
+
+Context {A: Type} (f: nat -> option A).
+
+Hypothesis f_mono: forall i j, i <= j -> f i <<= f j.
+
+Lemma limit_exists:
+  { lim : option A | exists i, forall j, i <= j -> f j = lim }.
+Proof.
+    apply constructive_definite_description.
+    destruct (classic (forall i, f i = None)) as [DIV|TERM].
+    - exists None; split.
+      + exists O; auto.
+      + intros lim (i & LIM). rewrite <- (DIV i). apply LIM; lia.
+    - apply not_all_ex_not in TERM. destruct TERM as (i & TERM).
+      exists (f i); split.
+      + exists i; intros. destruct (f_mono i j H). congruence. auto.
+      + intros lim (i2 & LIM2). set (j := Nat.max i i2).
+        rewrite <- (LIM2 j) by lia.
+        destruct (f_mono i j). lia. congruence. auto.
+Qed.
+
+Definition limit : option A := proj1_sig limit_exists.
+
+Lemma limit_charact: exists i, forall j, i <= j -> f j = limit.
+Proof. unfold limit. apply proj2_sig. Qed.
+
+End LIMIT.
+
+Definition option_bind {X Y: Type} (m : option X) (f: X -> option Y): option Y :=
+         match m with None => None | Some x => f x end.
+
+Definition option_lift {X Y: Type} (f: X -> Y): X -> option Y := fun x => Some (f x).
+
+Lemma option_bind_mono: forall (X Y: Type) (x x': option X) (f f': X -> option Y),
+    x <<= x' -> (forall x, f x <<= f' x) -> option_bind x f <<= option_bind x' f'.
+Proof. intros. destruct H; cbn; auto with lessdef. Qed.
+
+Fixpoint loop_fuel__C (fuel: nat) (f: Valuation -> option Valuation) (b: Bexpr) (V: Valuation): option Valuation :=
+         match fuel with
+        | 0 => None
+        | S n => if Beval V b
+                then option_bind (f V) (loop_fuel__C n f b)
+                else Some V
+        end.
+
+Lemma loop_mono: forall i j f b V,
+    i <= j -> loop_fuel__C i f b V <<= loop_fuel__C j f b V.
+Proof.
+    induction i; intros; simpl.
+    - constructor.
+    - destruct j.
+      + inversion H.
+      + simpl; destruct (Beval V b).
+        * apply option_bind_mono.
+          -- apply lessdef_refl.
+          -- intro. apply IHi. lia.
+        * constructor.
+Qed.
+
+(** Concrete semantics *)
+Definition loop__C (f: Valuation -> option Valuation) (b: Bexpr) (V: Valuation) : option Valuation :=
+         limit (fun n => loop_fuel__C n f b V) (fun i j => loop_mono i j f b V).
+
+Inductive denot__C: Stmt -> (Valuation -> option Valuation) -> Prop :=
+  | denot_skip__C: denot__C <{skip}> (fun V => Some V)
+  | denot_asgn__C: forall x e,
+      denot__C <{x := e}> (fun V => Some (x !-> Aeval V e; V))
+  | denot_seq__C: forall p1 p2 f1 f2,
+      denot__C p1 f1 ->
+      denot__C p2 f2 ->
+      denot__C <{p1 ; p2}> (fun V => option_bind (f1 V) f2)
+  | denot_if__C: forall b p1 p2 f1 f2,
+      denot__C p1 f1 ->
+      denot__C p2 f2 ->
+      denot__C <{if b {p1} {p2}}> (fun V => if Beval V b then f1 V else f2 V)
+  | denot_loop__C: forall b p f,
+      denot__C p f ->
+      denot__C <{while b {p}}> (loop__C f b)
+.
+
+Fixpoint denot_fun (p: Stmt) (V: Valuation): option Valuation :=
+         match p with
+        | <{skip}> => Some V
+        | <{x := e}> => Some (x !-> Aeval V e ; V)
+        | <{p1 ; p2}> => option_bind (denot_fun p1 V) (denot_fun p2)
+        | <{if b {p1} {p2}}> => if Beval V b then (denot_fun p1 V) else (denot_fun p2 V)
+        | <{while b {p}}> => loop__C (denot_fun p) b V
+         end.
+
+(* Characterizing the concrete denotation *)
+Lemma loop_charact__C: forall f b V, exists i, forall j, i <= j -> loop_fuel__C j f b V = loop__C f b V.
+Proof. intros. apply limit_charact. Qed.
+
+Lemma loop_unique__C: forall f b V i lim,
+    (forall j, i <= j -> loop_fuel__C j f b V = lim) ->
+    loop__C f b V = lim.
+Proof.
+    intros. destruct (loop_charact__C f b V) as [i' LIM].
+    set (j := Nat.max i i').
+    rewrite <- (H j). rewrite (LIM j). reflexivity.
+    all: lia.
+Qed.
+
+Lemma denot_seq: forall p1 p2 V,
+    denot_fun <{p1 ; p2}> V = option_bind (denot_fun p1 V) (denot_fun p2).
+Proof. reflexivity. Qed.
+
+Lemma denot_loop: forall f b V,
+    loop__C f b V = if Beval V b then option_bind (f V) (loop__C f b) else Some V.
+Proof.
+    intros.
+    destruct (f V) eqn:H.
+    - destruct (loop_charact__C f b v) as [i LIM].
+      apply loop_unique__C with (i := (S i)). intros.
+      destruct j; [lia|].
+      simpl. destruct (Beval V b);
+        try reflexivity.
+      rewrite H; cbn. apply LIM. lia.
+    - destruct (loop_charact__C f b V) as [i LIM].
+      apply loop_unique__C with (i := (S i)). intros.
+      destruct j; [lia|].
+      simpl. destruct (Beval V b);
+        [rewrite H|]; reflexivity.
+Qed.
+
+Lemma loop_false: forall f b V, Beval V b = false -> loop__C f b V = Some V.
+Proof. intros. rewrite denot_loop. rewrite H. reflexivity. Qed.
+
+Definition option_apply {A B: Type}: option (A -> B) -> A -> option B :=
+  fun f a => match f with
+          | None => None
+          | Some f => Some (f a)
+          end.
+
+Compute option_apply (denot_fun
+                      <{if X <= 10 {X := X + 1;
+                                       if X <= 5 {Y := X + X}
+                                              { skip }}
+                               { Y := 42 }}>
+                        (_ !-> 11)) Y.
+
+Compute option_apply (denot_fun
+                      <{while X <= 10 {X := X + 1;
+                                       if X <= 5 {Y := X + X}
+                                                { skip }} }>
+                        (_ !-> 0)) X.
+(* this result is annoying, but meh *)
+
+Example branch_example: Stmt := <{
+    if X <= 0
+           {if 1 <= 0 {X := 42} {X := 0}}
+           {if 1 <= 0 {X := 42} {X := 1}}
+    }>.
+
+(** Symbolic Semantics *)
+
+Definition Branch: Type := (Valuation -> Valuation) * (Ensemble Valuation).
+
+Definition inverse_image {X: Type} (F: X -> X) (B: Ensemble X): Ensemble X := fun x => B (F x).
+Definition denot__B (b: Bexpr): Ensemble Valuation := fun V => Beval V b = true.
+
+Lemma denotB_true: forall V b, In _ (denot__B b) V <-> Beval V b = true.
+Proof. split; intros; apply H. Qed.
+
+Search (forall b, b <> true -> b = false).
+
+Lemma denotB_false: forall V b, In _ (Complement _ (denot__B b)) V <-> Beval V b = false.
+Proof.
+    split; intros.
+    - apply (not_true_is_false _ H).
+    - unfold Complement, In, denot__B. intro. rewrite H in H0. discriminate.
+Qed.
+
+Fixpoint n_fold {X: Type} (n: nat) (f: X -> X): X -> X :=
+         match n with
+        | 0 => fun x => x
+        | S n => fun x => f (n_fold n f x)
+         end.
+
+Lemma n_fold_inversion {X:Type}: forall n f (x: X), f (n_fold n f x) = n_fold (S n) f x.
+Proof. reflexivity. Qed.
+
+Lemma n_fold_step {X:Type}: forall n f (x y: X), n_fold (S n) f x = y -> exists z, n_fold n f x = z /\ f z = y.
+Proof.
+    induction n; intros; simpl in *.
+    - exists x. split; [reflexivity | apply H].
+    - exists (f (n_fold n f x)). split; [reflexivity | apply H].
+Qed.
+
+Definition loop_helper (body: Ensemble Branch) (b: Bexpr) (p: Stmt): Ensemble Branch -> Ensemble Branch :=
+       fun big_F => fun X => exists F B Fp Bp,
+           In _ big_F (F, B)
+           /\ In _ body (Fp, Bp)
+           /\ fst X = (fun V => F (Fp V))
+           /\ snd X = Intersection _ (denot__B b) (Intersection _ Bp (inverse_image Fp B)).
+
+Lemma loop_helper_step: forall n body b p F B X0,
+    In _ (n_fold (S n) (loop_helper body b p) X0) (F, B) ->
+    exists F' B', In _ (n_fold n (loop_helper body b p) X0) (F', B')
+             /\ loop_helper body b p (Singleton _ (F', B')) (F, B)
+.
+Proof.
+    intros.
+    destruct (n_fold_step n (loop_helper body b p) X0 (n_fold (S n) (loop_helper body b p) X0))
+      as [Y [H0 H1]]; [reflexivity|].
+    destruct H as [F' [B' [Fp [Bp [Hbody [Hloop [tmp0 tmp1]]]]]]].
+    simpl in tmp0, tmp1; subst.
+    exists F'. exists B'. repeat split.
+    - apply Hbody.
+    - exists F'. exists B'. exists Fp. exists Bp.
+      repeat split. apply Hloop.
+Qed.
+
+Inductive Big_Union {X} (Xs: Ensemble (Ensemble X)) : Ensemble X :=
+  | Big_U_intro: forall X x, In _ Xs X -> In _ X x -> In _ (Big_Union Xs) x.
+
+Definition Union_Fam {X I} (Fs: I -> Ensemble X) : Ensemble X :=
+         let Xs : Ensemble (Ensemble X) := fun X => exists i, Fs i = X
+         in Big_Union Xs.
+
+Fixpoint denot__S (p: Stmt): Ensemble Branch := match p with
+        | <{skip}> => Singleton _ (fun V => V, Full_set _)
+        | <{x := e}> => Singleton _ (fun V => (x !-> Aeval V e ; V), Full_set _)
+        | <{p ; q}> =>
+            fun X => exists Fp Fq Bp Bq,
+                In _ (denot__S p) (Fp, Bp)
+                /\ In _ (denot__S q) (Fq, Bq)
+                /\ (fst X = fun V => Fq (Fp V))
+                /\ snd X = Intersection _ Bp (inverse_image Fp Bq)
+        | <{if b {p} {q}}> =>
+            fun X =>
+              (exists F B,
+                  In _ (denot__S p) (F, B)
+                  /\ fst X = F
+                  /\ snd X = Intersection _ B (denot__B b))
+              \/
+                (exists F B,
+                    In _ (denot__S q) (F, B)
+                    /\ fst X = F
+                    /\ snd X = Intersection _ B (Complement _ (denot__B b)))
+        | <{while b {p}}> =>
+            Union_Fam (fun m => n_fold m (loop_helper (denot__S p) b p) (Singleton _ (fun V => V, Complement _ (denot__B b))))
+         end.
+
+Lemma loop_correct (p: Stmt)
+  (IHp : forall (F : Valuation -> Valuation) (B : Ensemble Valuation) (V : Valuation),
+      In Branch (denot__S p) (F, B) -> In Valuation B V -> exists V' : Valuation, F V = V' /\ denot_fun p V = Some V'):
+  forall n F B b,
+    In _ (n_fold n (loop_helper (denot__S p) b p)
+         (Singleton _ (fun V => V, Complement _ (denot__B b))))
+   (F, B) ->
+    forall V,
+      In _ B V ->
+      loop_fuel__C (S n) (denot_fun p) b V = option_lift F V.
+Proof.
+    induction n; intros.
+    - simpl in *. inversion H; subst.
+      rewrite denotB_false in H0. rewrite H0.
+      reflexivity.
+    - destruct (loop_helper_step _ _ _ _ _ _ _ H) as [? [? [Hsofar Hstep]]].
+      destruct Hstep as [F' [B' [Fbody [Bbody [? [? [? ?]]]]]]].
+      simpl in H3, H4; subst.
+      inversion H1; subst.
+      inversion H0; subst.
+      rewrite denotB_true in H3.
+      specialize (IHn _ _ _ Hsofar (Fbody V)).
+      replace (loop_fuel__C (S (S n)) (denot_fun p) b V) with
+        (option_bind (denot_fun p V) (loop_fuel__C (S n) (denot_fun p) b)).
+      unfold option_lift in *. rewrite <- IHn. cbn.
+      replace (denot_fun p V) with (Some (Fbody V)).
+      reflexivity.
+      + destruct (IHp _ _ V H2) as [V' [? ?]];
+          [inversion H4; subst; assumption |].
+        rewrite H5, H6. reflexivity.
+      + destruct H4. apply H5.
+      + simpl. rewrite H3. reflexivity.
+Qed.
+
+Lemma correct: forall p F B V,
+    In _ (denot__S p) (F, B) ->
+    In _ B V ->
+    exists V', F V = V' /\ denot_fun p V = Some V'.
+Proof.
+    induction p; intros.
+    - inversion H; subst.
+      exists V. split; reflexivity.
+    - inversion H; subst.
+      exists (x !-> Aeval V e; V). split; reflexivity.
+    - destruct H as [F1 [F2 [B1 [B2 [H1 [H2 [HF HB]]]]]]].
+      exists (F2 (F1 V)). split.
+      + simpl in HF. rewrite HF. reflexivity.
+      + simpl in *.
+        rewrite HB in H0. inversion H0; subst.
+        destruct (IHp1 F1 B1 V H1 H) as [V1 [? HV1]]. rewrite HV1.
+        destruct (IHp2 F2 B2 (F1 V) H2 H3) as [V2 [? HV2]].
+        simpl.
+        rewrite <- H4. rewrite HV2. rewrite H5.
+        reflexivity.
+    - simpl. destruct H; destruct (Beval V b) eqn:Hcond.
+      (* condition true, left branch*)
+      + destruct H as [F1 [B1 [H1 [HF HB]]]].
+        simpl in HB. rewrite HB in H0. inversion H0; subst.
+        destruct (IHp1 F B1 V H1 H) as [V1 [HF1 HV1]].
+        exists V1. split; assumption.
+      (* condition false, left branch => contradiction *)
+      + destruct H as [F1 [B1 [H1 [HF HB]]]].
+        simpl in HB. rewrite HB in H0. inversion H0; subst.
+        unfold denot__B, In in H2. rewrite H2 in Hcond.
+        discriminate.
+      (* condition true, right branch => contradiction*)
+      + destruct H as [F2 [B2 [H2 [HF HB]]]].
+        simpl in HB. rewrite HB in H0. inversion H0; subst.
+        unfold denot__B, In, Complement in H1.
+        exfalso. apply H1. apply Hcond.
+      (* condition false, right branch *)
+      + destruct H as [F2 [B2 [H2 [HF HB]]]].
+        simpl in HB. rewrite HB in H0. inversion H0; subst.
+        destruct (IHp2 F B2 V H2 H) as [V2 [HF2 HV2]].
+        exists V2. split; assumption.
+    - inversion H; subst; cbn.
+      destruct (loop_charact__C (denot_fun p) b V) as [i' LIM].
+      rewrite <- LIM with (j := S i'); [| lia].
+      destruct H1. destruct x; cbn in *.
+      + rewrite <- H1 in H2. inversion H2; subst.
+        exists V. split.
+        * reflexivity.
+        * rewrite denotB_false in H0. rewrite H0. reflexivity.
+      + exists (F V). split.
+        * reflexivity.
+        * rewrite n_fold_inversion in H1.
+          rewrite <- H1 in H2.
+          destruct (loop_helper_step _ _ _ _ _ _ _ H2) as [? [? [Hsofar Hstep]]].
+          destruct Hstep as [F' [B' [Fbody [Bbody [? [? [? ?]]]]]]].
+          simpl in H5, H6; subst.
+          inversion H3; subst.
+          inversion H0; subst. inversion H5; subst.
+          specialize (loop_correct p IHp _ _ _ _ Hsofar (Fbody V) H7). intro.
+          rewrite denotB_true in H1. rewrite H1.
+          destruct (IHp _ _ _ H4 H6) as [V' [? ?]].
+          rewrite H10; simpl. rewrite <- H9.
+          replace i' with (S x).
+          (* the symbolic and concrete execution take same number of steps *)
+          (* which is not strictly true, but should be admissible *)
+          unfold option_lift in H8. apply H8.
+Admitted.
+
+Example branch_1: denot__S branch_example (fun V => (X !-> 42 ; V), Empty_set _).
+Proof.
+    left. exists (fun V => (X !-> 42 ; V)). eexists. repeat split.
+    - left. exists (fun V => (X !-> 42 ; V)). eexists. repeat split.
+    - simpl. apply Extensionality_Ensembles. split.
+      + intros V H. inversion H.
+      + intros V H. inversion H; subst; inversion H0; inversion H3.
+Qed.
+
+Example branch_2: denot__S branch_example (fun V => (X !-> 42 ; V), Empty_set _).
+Proof.
+    right. eexists. eexists. repeat split.
+    - left. eexists. eexists. repeat split.
+    - simpl. apply Extensionality_Ensembles. split.
+      + intros V H. inversion H.
+      + intros V H. inversion H; subst; inversion H0; inversion H3.
+Qed.
+
+Example branch_3: denot__S branch_example (fun V => (X !-> 0 ; V), fun V => V X = 0).
+Proof.
+    left. eexists. eexists. repeat split.
+    - right. eexists. eexists. repeat split.
+    - apply Extensionality_Ensembles. split; intros V H.
+      + inversion H. split.
+        * split.
+          -- apply Full_intro.
+          -- intro. rewrite H1 in H0. inversion H0.
+        * rewrite H1. unfold denot__B, In. simpl. rewrite H1. reflexivity.
+      + inversion H. inversion H1. apply leb_complete in H4. inversion H4. reflexivity.
+Qed.
+
+Lemma leb_correct_neg: forall n m, n <=? m <> true -> ~ (n <= m).
+Proof. intros n m H contra. apply H. apply leb_correct. apply contra. Qed.
+
+Example branch_4: denot__S branch_example (fun V => (X !-> 1 ; V), fun V => V X > 0).
+Proof.
+    right. eexists. eexists. repeat split.
+    - right. eexists. eexists. repeat split.
+    - apply Extensionality_Ensembles. split; intros V H.
+      + inversion H; repeat split; intro; inversion H0.
+        * rewrite <- H1 in H3. discriminate.
+        * inversion H2.
+        * inversion H2. rewrite <- H0 in H5. discriminate.
+      + inversion H. unfold In. simpl.
+        unfold Complement, In, denot__B in H1. simpl in H1.
+        apply leb_correct_neg in H1. apply not_le in H1.
+        assumption.
+Qed.
+
+Example loop_example: Stmt :=
+         <{ while X <= 10 {X := X + 1} }>.
+
+Example loop_0: denot__S loop_example (fun V => V, fun V => V X > 10).
+Proof. cbn. unfold Union_Fam. eapply Big_U_intro with (X := Singleton _ (fun V => V, fun V => V X > 10)).
+       - exists 0.
+       assert (Complement _ (denot__B <{ X <= 10 }>) = fun V => V X > 10).
+         { apply Extensionality_Ensembles. repeat split; intros V H.
+           - unfold Complement, In, denot__B in H. simpl in H. apply leb_correct_neg in H.
+             apply not_le in H. apply H.
+           - intro H'. unfold In, denot__B in *. simpl in *. apply leb_complete in H'. lia.
+         }
+         cbn. rewrite H. reflexivity.
+       - reflexivity.
+Qed.
