BigStepTraces.v
@@ -1,0 +1,230 @@
+(** Trying to reimplement the concrete big-step semantics of Nakata & Uustalu *)
+
+From Coq Require Import
+                 Strings.String
+                 Bool.Bool
+                 Init.Datatypes
+                 Lists.Streams
+                 Classes.RelationClasses
+.
+
+From SymEx Require Import Expr.
+Import BasicExpr.
+
+From SymEx Require Import Maps.
+Import BasicMaps.
+
+From SymEx Require Import While.
+Open Scope com_scope.
+
+CoInductive trace {X:Type}: Type :=
+| TSingl: X -> @trace X
+| TCons: X -> @trace X -> @trace X.
+
+CoInductive infinite {X:Type}: @trace X -> Prop :=
+  | inf_intro: forall t x, infinite t -> infinite (TCons x t).
+
+CoInductive trace_bisim {X: Type}: @trace X -> @trace X -> Prop :=
+| bisim_singl: forall x x': X, trace_bisim (TSingl x) (TSingl x)
+| bisim_step: forall t t' x, trace_bisim t t' -> trace_bisim (TCons x t) (TCons x t').
+
+Global Instance trace_bisim_refl {X: Type}: Reflexive (@trace_bisim X).
+Proof. cofix CH; intros x; destruct x.
+       - constructor. exact x.
+       - constructor. apply CH.
+Qed.
+
+Global Instance trace_eq_sym {X: Type}: Symmetric (@trace_bisim X).
+Proof.
+  cofix CH; intros x y H. destruct x, y;
+    try (inversion H; subst; assumption).
+  inversion H; subst. constructor. apply (CH _ _ H1).
+Qed.
+
+Global Instance trace_eq_trans {X: Type}: Transitive (@trace_bisim X).
+Proof.
+  cofix CH; intros x y z H0 H1. destruct x, y, z;
+    try (inversion H0; inversion H1; subst; assumption).
+  inversion H1; subst; inversion H0; subst. constructor.
+  apply (CH x0 y z H3 H2).
+Qed.
+
+Notation " t '~' t'" := (trace_bisim t t')
+                          (at level 40).
+
+Lemma unfold_trace {X: Type}:
+  forall t:@trace X, t = match t with
+                    | TSingl x => TSingl x
+                    | TCons x t => TCons x t
+                    end.
+Proof. intros. destruct t; reflexivity. Qed.
+
+Inductive last_state {X:Type}: @trace X -> X -> Prop :=
+| Last: forall x, last_state (TSingl x) x
+| NotLast:  forall t x x', last_state t x -> last_state (TCons x' t) x.
+
+Definition trace__S := @trace sub.
+Definition trace__C := @trace Valuation.
+
+(* Big-Step Functional Semantics *)
+CoFixpoint sequence (k: Valuation -> trace__C) (t: trace__C): trace__C :=
+  match t with
+  | TSingl V => k V
+  | TCons V t' => TCons V (sequence k t')
+  end.
+
+CoFixpoint loop (k: Valuation -> trace__C) (p: Valuation -> bool) (V: Valuation): trace__C :=
+  if p V then
+    match k V with
+    | TSingl V' => TCons V' (loop k p V')
+    | TCons V' t => TCons V' (loopseq k p t)
+    end
+  else TSingl V
+with loopseq (k: Valuation -> trace__C) (p: Valuation -> bool) (t: trace__C): trace__C :=
+       match t with
+       | TSingl V => TCons V (loop k p V)
+       | TCons V t' => TCons V (loopseq k p t')
+       end.
+
+Fixpoint eval (p:Stmt) (V:Valuation) {struct p}: trace__C :=
+  match p with
+  | <{skip}> => TSingl V
+  | <{x := e}> => TCons V (TSingl (x !-> Aeval V e ; V))
+  | <{p ; q}> => sequence (eval p) (eval q V)
+  | <{if e {p} {q}}> => TCons V (if Beval V e then eval p V else eval q V)
+  | <{while e {p}}> => TCons V (loop (eval p) (fun V => Beval V e) V)
+  end.
+
+(* Big-Step Relational Semantics *)
+Reserved Notation " s , V '==>' t " (at level 40).
+Reserved Notation " s , t '==>*' t' " (at level 40).
+
+CoInductive denot__C: Stmt -> Valuation -> trace__C -> Prop :=
+| denot_asgn__C: forall x e V,
+    <{x := e}> , V ==> TCons V (TSingl (x !-> Aeval V e ; V))
+| denot_skip__C: forall V,
+    <{skip}>, V ==> TSingl V
+| denot_seq__C: forall p q V t t',
+    p, V ==> t -> q, t ==>* t' ->
+    <{p ; q}>, V ==> t'
+| denot_ift__C: forall V e p q t,
+    Beval V e = true ->
+    p, (TCons V (TSingl V)) ==>* t ->
+    <{if e {p} {q}}>, V ==> t
+| denot_iff__C: forall V e p q t,
+    Beval V e = false ->
+    q, (TCons V (TSingl V)) ==>* t ->
+    <{if e {p} {q}}>, V ==> t
+| denot_whilet__C: forall V e p t t',
+    Beval V e = true ->
+    p, (TCons V (TSingl V)) ==>* t ->
+    <{while e {p}}>, t ==>* t' ->
+    <{while e {p}}>, V ==> t'
+| denot_whilef__C: forall V e p,
+    Beval V e = false ->
+    <{while e {p}}>, V ==> TCons V (TSingl V)
+where " s , V '==>' t " := (denot__C s V t)
+with denot_star__C: Stmt -> trace__C -> trace__C -> Prop :=
+| denotNil: forall V p t,
+    p, V ==> t -> p, (TSingl V) ==>* t
+| denotCons: forall V p t t',
+    p, t ==>* t' -> p, (TCons V t) ==>* TCons V t'
+where " s , t '==>*' t' " := (denot_star__C s t t') .
+
+Lemma denot_nil__C: forall p V V', denot__C p V (TSingl V') -> V = V'.
+Proof.
+  induction p; intros V V' H; inversion H; subst; auto.
+  (* seq case *)
+  - inversion H5; subst.
+    rewrite (IHp1 _ _ H2). rewrite (IHp2 _ _ H0).
+    reflexivity.
+  (* if cases *)
+  - inversion H6.
+  - inversion H6.
+  (* loop case *)
+  - inversion H3; subst. inversion H6.
+Qed.
+
+Lemma denot_star_deterministic__C: forall p,
+    (forall V t t', p, V ==> t -> p, V ==> t' -> t ~ t') ->
+    forall t1 t2 t3 t4,
+      t1 ~ t2 -> p, t1 ==>* t3 -> p, t2 ==>* t4 -> t3 ~ t4.
+Proof.
+  intros p H. cofix CH.
+  intros ? ? ? ? H1 H2 H3.
+  inversion H2; subst.
+  - inversion H3; subst;
+      inversion H1; subst; apply (H _ _ _ H0 H4).
+  - inversion H3; subst;
+      inversion H1; subst.
+    constructor. apply (CH _ _ _ _ H6 H0 H4).
+Qed.
+
+Lemma denot_seq_deterministic__C: forall p q,
+    (forall V t t', p, V ==> t -> p, V ==> t' -> t ~ t') ->
+    (forall V t t', q, V ==> t -> q, V ==> t' -> t ~ t') ->
+    forall V t t',
+      <{p;q}>, V ==> t ->
+      <{p;q}>, V ==> t' ->
+      t ~ t'.
+Proof.
+  intros. inversion H1; subst; inversion H2; subst.
+  specialize (H _ _ _ H5 H6).
+  apply (denot_star_deterministic__C _ H0 _ _ _ _ H H8 H10).
+Qed.
+
+
+Lemma denot_loop_star_deterministic__C: forall e p,
+  forall t1 t2 t3 t4,
+    t1 ~ t2 ->
+    <{while e {p}}>, t1 ==>* t3 ->
+    <{while e {p}}>, t2 ==>* t4 ->
+    t3 ~ t4.
+Proof.
+  intros e p. cofix CH.
+  intros t1 t2 t3 t4 H1 H2 H3.
+  inversion H2; subst.
+  - inversion H3; subst.
+    + inversion H1; subst. inversion H0; subst.
+      * inversion H; subst.
+Admitted.
+
+Lemma denot_loop_deterministic__C: forall e p,
+    (forall V t t', p, V ==> t -> p, V ==> t' -> t ~ t') ->
+    forall V t t',
+      <{while e {p}}>, V ==> t ->
+      <{while e {p}}>, V ==> t' ->
+      t ~ t'.
+Proof.
+  intros e p Hloop. cofix CH.
+  assert (CH2: forall t1 t2 t3 t4,
+    t1 ~ t2 ->
+    <{while e {p}}>, t1 ==>* t3 ->
+    <{while e {p}}>, t2 ==>* t4 ->
+    t3 ~ t4).
+  { cofix CH2. intros t1 t2 t3 t4 h1 h2 h3. inversion h2; subst.
+    - inversion h3; subst.
+      + inversion h1; subst. inversion H; subst.
+        * inversion H0; subst.
+          --
+        * inversion H; subst.
+          --
+  }
+  intros. inversion H0; subst.
+  - inversion H1; subst.
+    + eapply (denot_loop_star_deterministic__C e p _ _ _ _ _ H8 H11).
+    + admit.
+  - inversion H1; subst.
+    + inversion H0; subst.
+      * eapply (denot_loop_star_deterministic__C e p _ _ _ _ _ H12 H9).
+      *
+    + admit.
+      +
+
+(* Lemma 1: relational evaluation is deterministic up to bisimilarity *)
+Theorem denot_deterministic__C: forall V p t t', trace_bisim t t' -> p, V ==> t -> p, V ==> t'.
+Proof.
+  intros. cofix CH.
+  inversion H0; subst.
+  -
+Qed.
