While.v
@@ -1,0 +1,29 @@
+From Coq Require Import Strings.String.
+From SymEx Require Import Expr.
+Import BasicExpr.
+
+Inductive Stmt : Type :=
+| SSkip
+| SAsgn (x:string) (e:Aexpr)
+| SSeq (s1 s2:Stmt)
+| SIf (b:Bexpr) (s1 s2:Stmt)
+| SWhile (b:Bexpr) (s:Stmt).
+
+Notation "'skip'" := SSkip (in custom com at level 80) : com_scope.
+Notation "x := y"  :=
+         (SAsgn x y)
+            (in custom com at level 0, x constr at level 0,
+             y at level 85, no associativity) : com_scope.
+Notation "x ; y" :=
+         (SSeq x y)
+           (in custom com at level 90, right associativity) : com_scope.
+Notation "'if' x '{' y '}' '{' z '}'" :=
+         (SIf x y z)
+           (in custom com at level 89, x at level 99,
+            y at level 99, z at level 99) : com_scope.
+Notation "'while' x '{' y '}'" :=
+         (SWhile x y)
+           (in custom com at level 89, x at level 99,
+            y at level 99) : com_scope.
+
+Open Scope com_scope.
